balance_left and balance_right implementation

LLVM_DS_RBT/Delete.thy
@@ -1,6 +1,11 @@
 theory Delete
-  imports Setup
+  imports 
+    Setup
+    Utilities
+    "Insert/Balance"
+    Free
 begin
+
 
 context rbt_impl
 begin
@@ -9,51 +14,355 @@ interpretation llvm_prim_arith_setup .
 interpretation llvm_prim_setup .
 
 
-partial_function (M) delete :: "
-  ('ki, 'val::llvm_rep) rbti \<Rightarrow> unit llM 
-" where "
-  delete tree_p = do {
-    if tree_p = null
-    then return ()
-    else do {
-      tree \<leftarrow> ll_load tree_p;
-      key_delete (rbt_node.key tree);
-      ll_free tree_p;
-      delete (rbt_node.left tree);
-      delete (rbt_node.right tree)
+abbreviation "bl_pat_1 \<equiv> Branch CP_R RVar RVar"
+abbreviation "bl_pat_2 \<equiv> Branch CP_B RVar RVar"
+abbreviation "bl_pat_3 \<equiv> Branch CP_R (Branch CP_B RVar RVar) RVar"
+
+fun rbt_balance_left_ad where
+  "rbt_balance_left_ad l key val r =
+    (
+      if matches_rbt_pattern bl_pat_1 l
+      then case l of (rbt.Branch color.R a k x b) \<Rightarrow>
+        rbt.Branch color.R (rbt.Branch color.B a k x b) key val r
+      else if matches_rbt_pattern bl_pat_2 r
+      then case r of (rbt.Branch color.B a s y b) \<Rightarrow> 
+        rbt_balance l key val (rbt.Branch color.R a s y b)
+      else if matches_rbt_pattern bl_pat_3 r
+      then case r of (rbt.Branch color.R (rbt.Branch color.B a s y b) t z c) \<Rightarrow>
+        rbt.Branch color.R (rbt.Branch color.B l key val a) s y (rbt_balance b t z (paint color.R c))
+      else rbt.Empty
+    )"
+
+lemma rbt_balance_left_ad_correct:
+  "rbt_balance_left_ad l k v r = rbt_balance_left l k v r"
+  apply(induction l k v r rule: RBT_Impl.balance_left.induct)
+  by auto
+
+
+subsection \<open>Cases\<close>
+
+
+definition "bl_case_1 l_p k v r_p \<equiv>
+  do {
+    set_color_p 1 l_p;
+    new (RBT_NODE 0 l_p k v r_p)
+  }"
+
+
+definition "bl_case_2 l_p k v r_p \<equiv> 
+  do {
+    set_color_p 0 r_p;
+    balance l_p k v r_p
+  }"
+
+
+definition "bl_case_3 l_p k v r_p \<equiv> 
+  do {
+    let bl=l_p; k=k; x=v in
+    do {
+      r \<leftarrow> ll_load r_p;
+      case r of (RBT_NODE r_col rl_p t z c) \<Rightarrow> 
+      do {
+        rl \<leftarrow> ll_load rl_p;
+        case rl of (RBT_NODE rl_col a s y b) \<Rightarrow>
+        do {
+          (if c \<noteq> null then set_color_p 0 c else return ());
+          balanced \<leftarrow> balance b t z c;
+          ll_store (RBT_NODE 1 bl k x a) rl_p;
+          ll_store (RBT_NODE 0 rl_p s y balanced) r_p;
+          return r_p
+        }
+      }
+    }
+  }"
+
+
+definition "balance_left l_p k v r_p \<equiv> 
+  do {
+    if! matches_rbt_pattern_i bl_pat_1 l_p
+    then! bl_case_1 l_p k v r_p
+    else! if! matches_rbt_pattern_i bl_pat_2 r_p
+    then! bl_case_2 l_p k v r_p
+    else! if! matches_rbt_pattern_i bl_pat_3 r_p
+    then! bl_case_3 l_p k v r_p
+    else! do { 
+      key_delete k;
+      free l_p; free r_p;
+      empty
+    }
+  }"
+
+
+lemmas [llvm_inline] = 
+  bl_case_1_def
+  bl_case_2_def
+  bl_case_3_def
+
+
+lemmas [llvm_code] = balance_left_def
+
+
+lemma balance_left_correct':
+  "
+    llvm_htriple
+    (\<upharpoonleft>rbt_assn l li ** \<upharpoonleft>key_assn k ki ** \<upharpoonleft>rbt_assn r ri)
+    (balance_left li ki v ri)
+    (\<lambda>x. \<upharpoonleft>rbt_assn (rbt_balance_left_ad l k v r) x)
+  "
+  unfolding 
+    balance_left_def
+    bl_case_1_def
+    bl_case_2_def
+    bl_case_3_def
+  apply vcg
+  subgoal (*case 1*)
+    apply resolve_rbt_pat_mat
+    apply vcg
+    unfolding rbt_assn_branch_def
+    apply vcg
+    done
+  subgoal (*case 2+*)
+    apply vcg
+    subgoal (*case 2*)
+      apply resolve_rbt_pat_mat
+      apply vcg
+      apply (erule close_rbt_assn, vcg_solve)
+      apply vcg
+      done
+    subgoal (*case 3+*)
+      apply vcg
+      subgoal (*case 3*)
+        apply resolve_rbt_pat_mat
+        apply vcg
+        subgoal (*paint null case*)
+          unfolding rbt_assn_branch_def
+          apply vcg
+          done
+        subgoal (*paint non-null case*)
+          apply vcg
+          apply STATE_extract_pure
+          apply (erule rbt_assn_non_null_unfold, auto)
+          apply vcg
+          apply (erule close_rbt_assn, vcg_solve)
+          apply vcg
+          unfolding rbt_assn_branch_def
+          apply vcg
+          done
+        done
+      subgoal (*case 4*) by vcg
+      done
+    done
+  done
+
+lemma balance_left_correct [vcg_rules]:
+  "
+    llvm_htriple
+    (\<upharpoonleft>rbt_assn l li ** \<upharpoonleft>key_assn k ki ** \<upharpoonleft>rbt_assn r ri)
+    (balance_left li ki v ri)
+    (\<lambda>x. \<upharpoonleft>rbt_assn (rbt_balance_left l k v r) x)
+  "
+  using balance_left_correct' rbt_balance_left_ad_correct by metis
+
+
+subsection \<open>balance right\<close>
+
+
+subsubsection \<open>patterns\<close>
+
+abbreviation "br_pat_1 \<equiv> Branch CP_R RVar RVar"
+abbreviation "br_pat_2 \<equiv> Branch CP_B RVar RVar"
+abbreviation "br_pat_3 \<equiv> Branch CP_R RVar (Branch CP_B RVar RVar)"
+
+definition "br_case_1 l_p k v r_p \<equiv>
+  do {
+    set_color_p 1 r_p;
+    new (RBT_NODE 0 l_p k v r_p)
+  }"
+
+
+definition "br_case_2 l_p k v r_p \<equiv> 
+  do {
+    set_color_p 0 l_p;
+    balance l_p k v r_p
+  }"
+
+
+definition "br_case_3 l_p k v r_p \<equiv> 
+  do {
+    let bl=r_p; t=k; z=v in
+    do {
+      l \<leftarrow> ll_load l_p;
+      case l of (RBT_NODE l_col a k x lr_p) \<Rightarrow> 
+      do {
+        lr \<leftarrow> ll_load lr_p;
+        case lr of (RBT_NODE lr_col b s y c) \<Rightarrow>
+        do {
+          (if a \<noteq> null then set_color_p 0 a else return ());
+          balanced \<leftarrow> balance a k x b;
+          ll_store (RBT_NODE 1 c t z bl) lr_p;
+          ll_store (RBT_NODE 0 balanced s y lr_p) l_p;
+          return l_p
+        }
+      }
+    }
+  }"
+
+
+fun rbt_balance_right_ad where   
+  "rbt_balance_right_ad l key val r =
+    (
+      if matches_rbt_pattern br_pat_1 r
+      then case r of (rbt.Branch color.R a k x b) \<Rightarrow>
+        rbt.Branch color.R l key val (rbt.Branch color.B a k x b)
+      else if matches_rbt_pattern br_pat_2 l
+      then case l of (rbt.Branch color.B a s y b) \<Rightarrow> 
+        rbt_balance (rbt.Branch color.R a s y b) key val r
+      else if matches_rbt_pattern br_pat_3 l
+      then case l of (rbt.Branch color.R a k x (rbt.Branch color.B b s y c)) \<Rightarrow>
+        rbt.Branch color.R (rbt_balance (paint color.R a) k x b) s y (rbt.Branch color.B c key val r)
+      else rbt.Empty
+    )"
+  
+lemma rbt_balance_right_ad_correct:
+  "rbt_balance_right_ad l k v r = rbt_balance_right l k v r"
+  apply (induction l k v r rule: RBT_Impl.balance_right.induct)
+  apply auto
+  done
+
+definition "balance_right l_p k v r_p \<equiv>
+  do {
+    if! matches_rbt_pattern_i br_pat_1 r_p
+    then! br_case_1 l_p k v r_p
+    else! if! matches_rbt_pattern_i br_pat_2 l_p
+    then! br_case_2 l_p k v r_p
+    else! if! matches_rbt_pattern_i br_pat_3 l_p
+    then! br_case_3 l_p k v r_p
+    else! do { 
+      key_delete k;
+      free l_p; free r_p;
+      empty
     }
   }
 "
 
-
-lemma delete_rule [vcg_rules]: "
-  llvm_htriple
-  (\<upharpoonleft>rbt_assn tree treei)
-  (delete treei)
-  (\<lambda>_. \<box>)
-"
-proof(induction tree arbitrary: treei)
-  case Empty
-  then show ?case
-    apply (subst delete.simps)
-    apply vcg_monadify
+lemma balance_right_correct':
+  "
+    llvm_htriple
+    (\<upharpoonleft>rbt_assn l li ** \<upharpoonleft>key_assn k ki ** \<upharpoonleft>rbt_assn r ri)
+    (balance_right li ki v ri)
+    (\<lambda>x. \<upharpoonleft>rbt_assn (rbt_balance_right_ad l k v r) x)
+  "
+  unfolding
+    balance_right_def
+    br_case_1_def
+    br_case_2_def
+    br_case_3_def
+  apply vcg
+  subgoal (*case 1*)
+    apply resolve_rbt_pat_mat
+    apply vcg
+    unfolding rbt_assn_branch_def
     apply vcg
     done
-next
-  case (Branch col lhs k v rhs)
-
-  note [vcg_rules] = Branch.IH 
-  note [simp] = rbt_assn_branch_def
-  
-  then show ?case
-    apply (subst delete.simps)
-    apply vcg_monadify
+  subgoal (*case 2+*)
     apply vcg
+    subgoal (*case 2*) 
+      apply resolve_rbt_pat_mat
+      apply vcg
+      apply (erule close_rbt_assn, vcg_solve)
+      apply vcg
+      done
+    subgoal (*case 3+*)
+      apply vcg
+      subgoal (*case 3*)
+        apply resolve_rbt_pat_mat        
+        apply vcg
+        subgoal (*paint null*)
+          unfolding rbt_assn_branch_def
+          apply vcg
+          done
+        subgoal (*paint non-null*)
+          apply standard
+          apply STATE_extract_pure
+          apply (erule rbt_assn_non_null_unfold, auto)
+          apply vcg
+          apply (erule close_rbt_assn, vcg_solve)
+          apply vcg
+          unfolding rbt_assn_branch_def
+          apply vcg
+          done
+        done
+      subgoal (*case 4*) by vcg
+      done
     done
-qed
+  done
+
+lemma balance_right_correct [vcg_rules]:
+  "
+    llvm_htriple
+    (\<upharpoonleft>rbt_assn l li ** \<upharpoonleft>key_assn k ki ** \<upharpoonleft>rbt_assn r ri)
+    (balance_right li ki v ri)
+    (\<lambda>x. \<upharpoonleft>rbt_assn (rbt_balance_right l k v r) x)
+  "
+  using balance_right_correct' rbt_balance_right_ad_correct by metis
 
 
-end
+lemmas [llvm_inline] = 
+  br_case_1_def
+  br_case_2_def
+  br_case_3_def
+
+
+lemmas [llvm_code] = balance_right_def
+
+
+subsection \<open>random crap\<close>
+
+
+definition "Equiv (f:: real \<Rightarrow> real) g \<equiv> \<forall>x. f (g x) = x"
+
+
+lemma 1 [intro]: "f = (\<lambda>x. f' (x - c)) \<Longrightarrow> Equiv f' g \<Longrightarrow> Equiv f (\<lambda>x. g x + c)"
+  unfolding Equiv_def by simp
+
+lemma 2 [intro]: "Equiv f (\<lambda>x. g x + (-c)) \<Longrightarrow> Equiv f (\<lambda>x. g x - c)"
+  by simp
+
+lemma 3 [intro]: "c \<noteq> 0 \<Longrightarrow> f = (\<lambda>x. f' ( x / c)) \<Longrightarrow> Equiv f' g \<Longrightarrow> Equiv f (\<lambda>x. c * g x)"
+  unfolding Equiv_def
+  by auto
+
+lemma 4 [intro]: "f = (\<lambda>x. x) \<Longrightarrow> Equiv f (\<lambda>x. x)"
+  unfolding Equiv_def by simp
+
+lemma 5 [intro]: "Equiv f (\<lambda>x. (1/c) * g x ) \<Longrightarrow> Equiv f (\<lambda>x. g x / c)"
+  by simp
+
+
+
+definition "g \<equiv> (\<lambda>(x::real). 2 * (x + 5 - x) + x + 12 * x - 1 + (1.1 * x))"
+
+schematic_goal "Equiv ?f g"
+  unfolding g_def
+  apply (rule | simp)+
+  done
+
+
+definition "Cond (ff::'a list \<Rightarrow> 'b) (gg:: 'a list \<Rightarrow> 'b) = (ff = gg)"
+
+
+lemma R1: "f [] = undefined \<Longrightarrow> (\<And>l. f l = E (hd l) (tl l)) \<Longrightarrow> Cond f (\<lambda>l. case l of x # xs \<Rightarrow> E x xs)" 
+  unfolding Cond_def
+  apply standard
+  by (simp add: list.case_eq_if)
+
+
+schematic_goal "Cond ?f (\<lambda>l. case l of x # (y # xs) \<Rightarrow> x)"
+  apply (rule R1)
+  sorry
+
+
+end 
 
 
 end
