LLVM_DS_RBT/Abstract_Rbt.thy
@@ -1,0 +1,78 @@
+theory Abstract_Rbt
+  imports "HOL-Library.RBT_Impl"
+begin
+
+abbreviation "rbt_balance \<equiv> RBT_Impl.balance"
+abbreviation "rbt_balance_left \<equiv> RBT_Impl.balance_left"
+abbreviation "rbt_balance_right \<equiv> RBT_Impl.balance_right"
+
+hide_const balance
+hide_const balance_left
+hide_const balance_right
+
+
+subsection \<open>Rbt Utilities\<close>
+
+
+definition "rbt_is_red tree \<equiv> 
+  case tree of
+    (Branch color.R _ _ _ _ ) \<Rightarrow> True |
+    _ \<Rightarrow> False
+"
+
+
+lemma rbt_is_red_unfold_branch [elim!]:
+  assumes "rbt_is_red tree"
+  obtains lhs k v rhs where "tree = Branch color.R lhs k v rhs"
+  using assms
+  unfolding rbt_is_red_def
+  apply (cases tree)
+  subgoal by auto
+  subgoal for c  by (cases c; auto)
+  done
+
+
+definition "rbt_is_black tree \<equiv> 
+  case tree of
+    (rbt.Branch color.B _ _ _ _ ) \<Rightarrow> True |
+    rbt.Empty \<Rightarrow> True |
+    _ \<Rightarrow> False
+"
+
+
+lemma rbt_is_black_cases [elim!]:
+  assumes
+    "rbt_is_black tree"
+    "tree = rbt.Empty \<Longrightarrow> thesis"
+    "EX l k v r. tree = (rbt.Branch color.B l k v r) \<Longrightarrow> thesis"
+  shows "thesis"
+  using assms
+  unfolding rbt_is_black_def
+  by (auto split: color.splits rbt.splits)
+  
+
+lemma rbt_is_black_branchE [elim!]:
+  assumes 
+    "rbt_is_black (rbt.Branch c l k v r)"
+    "c = color.B \<Longrightarrow> thesis"
+  shows "thesis"
+  using assms by auto
+
+
+definition "rbt_is_branch tree \<equiv> 
+  (case tree of rbt.Empty \<Rightarrow> False | _ \<Rightarrow> True)"
+
+
+lemma rbt_is_branch_unfold [elim!]:
+  assumes "rbt_is_branch tree"
+  obtains c lhs k v rhs where "tree = Branch c lhs k v rhs"
+  using assms
+  unfolding rbt_is_branch_def
+  by (cases tree; auto)
+
+
+definition "rbt_left node \<equiv> case node of (Branch _ lhs _ _ _) \<Rightarrow> lhs" 
+definition "rbt_right node \<equiv> case node of (Branch _ _ _ _ rhs) \<Rightarrow> rhs"
+
+
+end
