LLVM_DS_RBT/Free.thy
@@ -1,0 +1,60 @@
+theory Free
+  imports Setup
+begin
+
+context rbt_impl
+begin
+interpretation llvm_prim_ctrl_setup .
+interpretation llvm_prim_arith_setup .
+interpretation llvm_prim_setup .
+
+
+partial_function (M) free :: "
+  ('ki, 'val::llvm_rep) rbti \<Rightarrow> unit llM 
+" where "
+  free tree_p = do {
+    if tree_p = null
+    then return ()
+    else do {
+      tree \<leftarrow> ll_load tree_p;
+      key_delete (rbt_node.key tree);
+      ll_free tree_p;
+      free (rbt_node.left tree);
+      free (rbt_node.right tree)
+    }
+  }
+"
+
+
+lemma free_correct [vcg_rules]: "
+  llvm_htriple
+  (\<upharpoonleft>rbt_assn tree treei)
+  (free treei)
+  (\<lambda>_. \<box>)
+"
+proof(induction tree arbitrary: treei)
+  case Empty
+  then show ?case
+    apply (subst free.simps)
+    apply vcg
+    done
+next
+  case (Branch col lhs k v rhs)
+
+  note [vcg_rules] = Branch.IH 
+  note [simp] = rbt_assn_branch_def
+  
+  then show ?case
+    apply (subst free.simps)
+    apply vcg
+    done
+qed
+
+
+lemmas [llvm_code] = free.simps
+
+
+end
+
+
+end
