LLVM_DS_RBT/Utilities.thy
@@ -1,0 +1,408 @@
+theory Utilities
+  imports Setup
+begin
+
+
+context rbt_impl
+begin
+interpretation llvm_prim_ctrl_setup .
+interpretation llvm_prim_arith_setup .
+interpretation llvm_prim_setup .
+
+
+lemma pure_part_split_conjE:
+  fixes A B
+  assumes "pure_part (A ** B)"
+  obtains
+    "pure_part A"
+    "pure_part B"
+  using assms
+  by (blast dest: pure_part_split_conj)
+
+lemma rbt_assn_non_null_def:
+  assumes 
+    "pure_part (\<upharpoonleft>rbt_assn t ti)"
+  shows
+    "ti = null \<longleftrightarrow> (t = rbt.Empty)"
+  using assms
+  apply (cases t)
+  subgoal by simp
+  subgoal
+    unfolding rbt_assn_branch_def
+    by fastforce
+  done
+
+lemma rbt_assn_non_null_unfold:
+  assumes 
+    "ti \<noteq> null"
+    "pure_part (\<upharpoonleft>rbt_assn t ti)"
+  obtains c l k v r where
+  "t = (rbt.Branch c l k v r)"
+  using assms rbt_assn_non_null_def
+  by (cases t; auto)
+
+lemma extract_pure: "STATE asf X s \<Longrightarrow> (pure_part X \<Longrightarrow> thesis) \<Longrightarrow> thesis"
+  by (meson STATE_def pure_partI)
+
+
+
+
+subsubsection \<open>Macros\<close>
+
+
+definition If_ll :: 
+  "1 word llM \<Rightarrow> 'a llM \<Rightarrow> 'a llM \<Rightarrow> 'a llM" 
+  ("(if! (_)/ then! (_)/ else! (_))" [0, 0, 10] 10) where
+  "If_ll condf truef elsef = do {
+    cond \<leftarrow> condf;
+    if cond = 1
+    then truef
+    else elsef
+  }"
+
+
+definition sc_and (infixl "&&!" 35) where
+  "sc_and a b \<equiv> do {
+    if! a
+    then! b
+    else! return 0
+  }"
+
+
+definition sc_or (infixl "||!" 30) where
+  "sc_or a b \<equiv> do {
+    if! a
+    then! return 1
+    else! b
+  }"
+
+
+lemmas [simp, llvm_pre_simp] = If_ll_def sc_and_def sc_or_def
+
+
+subsection \<open>Functions\<close>
+
+
+definition "is_red node_p \<equiv> do {
+    if node_p = null
+    then return 0
+    else do {
+      node \<leftarrow> ll_load node_p;
+      return from_bool (rbt_node.color node = 0)
+    }
+  }"
+
+
+lemma is_red_correct [vcg_rules]:
+  "
+    llvm_htriple
+    (\<upharpoonleft>rbt_assn t ti)
+    (is_red ti)
+    (\<lambda>r. \<up>(r = fb (rbt_is_red t)) ** \<upharpoonleft>rbt_assn t ti) 
+  "
+proof(cases t)
+  case Empty
+  then show ?thesis 
+    unfolding is_red_def rbt_is_red_def
+    by vcg
+next
+  case (Branch col lhs k v rhs)
+  then show ?thesis
+    apply (simp add: rbt_assn_branch_def rbt_is_red_def is_red_def)
+    apply (cases col)
+    apply vcg
+    done
+qed
+
+
+definition "left node_p \<equiv> do {
+    node \<leftarrow> ll_load node_p;
+    return rbt_node.left node
+}"
+
+
+lemma left_correct [vcg_rules]:
+  "
+    llvm_htriple
+    (\<upharpoonleft>rbt_assn (Branch col lhs k v rhs) ni)
+    (left ni)
+    (\<lambda>lhsi.
+      EXS coli ki vi rhsi. 
+        \<upharpoonleft>ll_bpto (RBT_NODE coli lhsi ki vi rhsi) ni **
+        \<upharpoonleft>color_assn col coli **
+        \<upharpoonleft>rbt_assn lhs lhsi **
+        \<upharpoonleft>key_assn k ki **
+        \<up>(vi=v) **  
+        \<upharpoonleft>rbt_assn rhs rhsi
+    )
+  "
+  unfolding left_def
+  by vcg
+
+
+definition "right node_p \<equiv> do {
+    node \<leftarrow> ll_load node_p;
+    return rbt_node.right node
+}"
+
+
+lemma right_correct [vcg_rules]:
+  "
+    llvm_htriple
+    (\<upharpoonleft>rbt_assn (Branch col lhs k v rhs) ni)
+    (right ni)
+    (\<lambda>rhsi.
+      EXS coli lhsi ki vi. 
+        \<upharpoonleft>ll_bpto (RBT_NODE coli lhsi ki vi rhsi) ni **
+        \<upharpoonleft>color_assn col coli **
+        \<upharpoonleft>rbt_assn lhs lhsi **
+        \<upharpoonleft>key_assn k ki **
+        \<up>(vi=v) **  
+        \<upharpoonleft>rbt_assn rhs rhsi
+    )
+  "
+  unfolding right_def
+  by vcg
+
+
+definition "is_branch node_p \<equiv> Mreturn (from_bool (node_p \<noteq> null))"
+
+
+lemma is_branch_correct [vcg_rules]:
+  "
+    llvm_htriple
+    (\<upharpoonleft>rbt_assn t ti)
+    (is_branch ti)
+    (\<lambda>r. \<up>(r = fb (rbt_is_branch t)) ** \<upharpoonleft>rbt_assn t ti) 
+  "
+  unfolding is_branch_def rbt_is_branch_def
+  by (cases t; vcg)
+
+
+definition "is_black node_p \<equiv>
+  Mreturn (from_bool (node_p = null)) ||!
+  do {
+    node \<leftarrow> ll_load node_p;
+    return from_bool (rbt_node.color node = 1)
+  }"
+
+
+lemma is_black_correct [vcg_rules]:
+  "
+    llvm_htriple
+    (\<upharpoonleft>rbt_assn t ti)
+    (is_black ti)
+    (\<lambda>r. \<up>(r = fb (rbt_is_black t)) ** \<upharpoonleft>rbt_assn t ti) 
+  "
+  unfolding is_black_def rbt_is_black_def
+  apply (cases t; (auto split: color.splits))
+    apply vcg
+  unfolding rbt_assn_branch_def
+   apply vcg
+  done
+
+
+definition "is_black_branch node_p \<equiv> 
+  Mreturn (from_bool (node_p \<noteq> null)) &&! 
+  do {
+    node \<leftarrow> ll_load node_p;
+    return from_bool (rbt_node.color node = 1)
+  }"
+
+
+lemma is_black_branch_correct [vcg_rules]:
+  "
+    llvm_htriple
+    (\<upharpoonleft>rbt_assn t ti)
+    (is_black_branch ti)
+    (\<lambda>r. \<up>(r = fb (rbt_is_black t \<and> rbt_is_branch t)) ** \<upharpoonleft>rbt_assn t ti) 
+  "
+  unfolding is_black_branch_def rbt_is_black_def rbt_is_branch_def
+  apply (cases t; (auto split: color.splits))
+    apply vcg
+  unfolding rbt_assn_branch_def
+   apply vcg
+  done
+
+
+
+definition "new x \<equiv> do {
+    ptr \<leftarrow> ll_balloc;
+    ll_store x ptr;
+    return ptr
+  }"
+
+
+lemma new_correct [vcg_rules]:
+  "
+    llvm_htriple
+    \<box>
+    (new x)
+    (\<lambda>r. \<upharpoonleft>ll_bpto x r)
+  "
+  unfolding new_def
+  by vcg
+
+
+lemmas [llvm_inline] = 
+  is_red_def
+  left_def
+  right_def
+  new_def
+
+datatype ColorPattern = CP_Var | CP_R | CP_B
+datatype RbtPattern = RVar | Empty | Branch ColorPattern RbtPattern RbtPattern
+
+fun matches_color_pattern_i ::
+  "ColorPattern \<Rightarrow> 8 word \<Rightarrow> 1 word llM" where
+  "matches_color_pattern_i CP_Var c = Mreturn ll_True"
+| "matches_color_pattern_i CP_R c = Mreturn (fb (c = 0))"
+| "matches_color_pattern_i CP_B c = Mreturn (fb (c = 1))"
+
+
+fun matches_color_pattern ::
+  "ColorPattern \<Rightarrow> color \<Rightarrow> bool" where
+  "matches_color_pattern CP_Var c = True"
+| "matches_color_pattern CP_R c = (c = color.R)"
+| "matches_color_pattern CP_B c = (c = color.B)"
+  
+
+fun matches_rbt_pattern ::
+  "RbtPattern \<Rightarrow> ('k, 'v) rbt \<Rightarrow> bool" where
+  "matches_rbt_pattern RVar t = True"
+| "matches_rbt_pattern Empty t = (t = rbt.Empty)"
+| "matches_rbt_pattern (Branch c l r) rbt.Empty = False"
+| "matches_rbt_pattern (Branch cp lp rp) (rbt.Branch c l _ _ r) = 
+  (matches_color_pattern cp c \<and> matches_rbt_pattern lp l \<and> matches_rbt_pattern rp r)"
+
+
+fun matches_rbt_pattern_i ::
+  "RbtPattern \<Rightarrow> ('ki, 'v::llvm_rep) rbti \<Rightarrow> 1 word llM" where
+  "matches_rbt_pattern_i RVar t = Mreturn ll_True"
+| "matches_rbt_pattern_i Empty t = Mreturn (fb(t = null))"
+| "matches_rbt_pattern_i (Branch c l r) t = do {
+    if t = null then return ll_False
+    else do {
+      node \<leftarrow> ll_load t;
+      case node of (RBT_NODE ci li ki v ri) \<Rightarrow> 
+      do {
+        c_check \<leftarrow> matches_color_pattern_i c ci;
+        l_check \<leftarrow> matches_rbt_pattern_i l li;
+        r_check \<leftarrow> matches_rbt_pattern_i r ri;
+        return c_check && l_check && r_check
+      }
+    }
+  }"
+
+lemma H1: "\<flat>\<^sub>pcolor_assn c ci \<Longrightarrow> fb (ci = 0) = fb (c = color.R)"
+  by (smt (verit) color.exhaust color.simps(3) color.simps(4) color_assn_eq dr_assn_pure_asm_prefix_def pure_part_pureD zero_neq_one)
+
+
+lemma H2: "\<flat>\<^sub>pcolor_assn c ci \<Longrightarrow> fb (ci = 1) = fb (c = color.B)"
+  by (smt (verit) color.exhaust color.simps(3) color.simps(4) color_assn_eq dr_assn_pure_asm_prefix_def pure_part_pureD zero_neq_one)
+
+lemma matches_color_pattern_correct [vcg_rules]:
+"
+  llvm_htriple
+  (\<upharpoonleft>color_assn c ci)
+  (matches_color_pattern_i pat ci)
+  (\<lambda>r. \<up>(r = fb (matches_color_pattern pat c)) )
+"
+  apply(cases pat)
+  using H1 H2 by vcg
+  
+
+lemma H3: "pure_part (\<upharpoonleft>rbt_assn t ti) \<Longrightarrow> fb (ti = null) = fb (t = rbt.Empty)"
+  apply (rule arg_cong[where f = fb])
+  apply (cases ti)
+  apply auto
+  done
+
+method STATE_extract_pure = 
+  rule extract_pure,
+  (auto)[1],
+  ((erule pure_part_split_conjE)+)?
+
+
+lemma fb_and [simp]: "fb x && fb y = fb (x \<and> y)"
+  unfolding fb_def 
+  using llvm_from_bool_inline(1) by metis
+
+
+lemma matches_rbt_pattern_correct [vcg_rules]:
+"
+  llvm_htriple
+  (\<upharpoonleft>rbt_assn t ti)
+  (matches_rbt_pattern_i pat ti)
+  (\<lambda>r. \<up>(r = fb (matches_rbt_pattern pat t)) ** \<upharpoonleft>rbt_assn t ti)
+"
+proof(induction pat arbitrary: t ti)
+  case RVar
+  then show ?case by vcg
+next
+  case Empty
+  then show ?case 
+    using H3 by vcg 
+next
+  case (Branch x1 pat1 pat2)
+
+  note [vcg_rules] = Branch
+  
+  show "?case"
+    apply vcg
+    apply STATE_extract_pure
+    apply (rule rbt_assn_non_null_unfold, auto)
+    apply vcg
+    apply auto
+    unfolding rbt_assn_branch_def
+    by vcg
+qed
+
+
+lemma matches_rbt_pattern_var_E:
+  assumes 
+    "matches_rbt_pattern RVar t" and 
+    "thesis"
+  shows "thesis"
+  using assms by simp
+
+
+lemma matches_rbt_pattern_empty_E:
+  assumes 
+    "matches_rbt_pattern Empty t" and 
+    "t = rbt.Empty \<Longrightarrow> thesis"
+  shows "thesis"
+  using assms by simp
+
+
+lemma matches_rbt_pattern_branch_E:
+  assumes                  
+    "matches_rbt_pattern (Branch cp lp rp) t" 
+  obtains c l k v r
+  where 
+    "t = rbt.Branch c l k v r" and
+    "matches_color_pattern cp c" and
+    "matches_rbt_pattern lp l" and
+    "matches_rbt_pattern rp r"
+  using assms by (cases t, auto)
+
+
+lemmas matches_rbt_pattern_unfold_elims = 
+  matches_rbt_pattern_var_E
+  matches_rbt_pattern_empty_E
+  matches_rbt_pattern_branch_E
+
+lemmas [simp del] = matches_rbt_pattern_i.simps
+
+lemmas [llvm_pre_simp] =
+  matches_rbt_pattern_i.simps
+  matches_color_pattern_i.simps
+  fb_def
+
+method resolve_rbt_pat_mat =
+  (auto elim!: matches_rbt_pattern.elims(1-2))[1]
+
+end
+
+
+end
